@prefix IAO: <http://purl.obolibrary.org/obo/IAO_> .
@prefix dcterms: <http://purl.org/dc/terms/> .
@prefix linkml: <https://w3id.org/linkml/> .
@prefix owl: <http://www.w3.org/2002/07/owl#> .
@prefix rdfs: <http://www.w3.org/2000/01/rdf-schema#> .
@prefix skos: <http://www.w3.org/2004/02/skos/core#> .
@prefix xsd: <http://www.w3.org/2001/XMLSchema#> .

<https://example.org/TEMP/Checklists> a owl:Class,
        linkml:ClassDefinition ;
    rdfs:label "Checklists" ;
    rdfs:subClassOf <https://example.org/TEMP/Biosample> ;
    skos:definition "A representation of required terms, according to the type of sequencing to be performed and the types of organisms expected to be found" .

<https://example.org/TEMP/Extension> a owl:Class,
        linkml:ClassDefinition ;
    rdfs:label "Extension" ;
    rdfs:subClassOf <https://example.org/TEMP/Biosample> ;
    skos:definition "Most recently defined as a representation of the environment from which a Biosample could be obtained, and the corresponding relevant metadata terms." .

<https://example.org/TEMP/Package> a owl:Class,
        linkml:ClassDefinition ;
    rdfs:label "Package" ;
    rdfs:subClassOf <https://example.org/TEMP/Biosample> ;
    skos:definition "Most recently defined as the combination of a Checklist and an Extension" .

linkml:SubsetDefinition a owl:Class ;
    rdfs:label "subset_definition" .

linkml:TypeDefinition a owl:Class ;
    rdfs:label "type_definition" .

linkml:topValue a owl:DatatypeProperty ;
    rdfs:label "value" .

<https://w3id.org/microbiomedata/mixs_fresh_start> a owl:Ontology ;
    rdfs:label "mixs_fresh_start" ;
    IAO:0000700 <https://example.org/TEMP/Biosample> ;
    dcterms:license "MIT" ;
    dcterms:title "mixs_fresh_start" ;
    rdfs:seeAlso "https://microbiomedata.github.io/mixs_fresh_start" ;
    linkml:generation_date "2023-02-13T13:23:14" ;
    linkml:metamodel_version "1.7.0" ;
    linkml:source_file "mixs_fresh_start.yaml" ;
    linkml:source_file_date "2023-02-13T12:37:56" ;
    linkml:source_file_size 568 .

<https://example.org/TEMP/depth> a owl:ObjectProperty,
        linkml:SlotDefinition ;
    rdfs:label "depth" ;
    rdfs:range <https://example.org/TEMP/QuantityValue> ;
    skos:definition "the distance between some reference point, like average sea level, and the spot from which a sampe ws obtained" .

<https://example.org/TEMP/has_raw_value> a owl:ObjectProperty,
        linkml:SlotDefinition ;
    rdfs:label "has_raw_value" ;
    rdfs:range linkml:String ;
    skos:definition "the input provoded by a user" .

<https://example.org/TEMP/QuantityValue> a owl:Class,
        linkml:ClassDefinition ;
    rdfs:label "QuantityValue" ;
    rdfs:subClassOf [ a owl:Restriction ;
            owl:maxQualifiedCardinality 1 ;
            owl:onClass linkml:String ;
            owl:onProperty <https://example.org/TEMP/has_raw_value> ],
        <https://example.org/TEMP/Biosample> ;
    skos:definition "The NMDC-preferred structured representation of magnitude/unit pairs" .

linkml:SlotDefinition a owl:Class ;
    rdfs:label "slot_definition" .

<https://example.org/TEMP/Biosample> a owl:Class,
        linkml:ClassDefinition ;
    rdfs:label "Biosample" ;
    rdfs:subClassOf [ a owl:Restriction ;
            owl:maxQualifiedCardinality 1 ;
            owl:onClass <https://example.org/TEMP/QuantityValue> ;
            owl:onProperty <https://example.org/TEMP/depth> ] ;
    skos:definition "An implied root of all MIxS classes (Packages? EnvironmentalPackages?,) Possibly abstract. Never actually mentioned in any MIxS literature." .

linkml:ClassDefinition a owl:Class ;
    rdfs:label "class_definition" .


